refactoring definition

lawyer/nonblocking/trace_context.v
@@ -1,19 +1,56 @@
 From trillium.traces Require Import exec_traces trace_lookup. 
 From trillium.program_logic Require Import language adequacy.
+From fairness Require Import locales_helpers. 
+
+
+Section ThreadPoolContext.
+  Context {Λ: language}. 
+  Context `{EqDecision (locale Λ)}. 
+
+  Record tpool_ctx := TpoolCtx {
+    tpctx_ctx: ectx Λ;
+    tpctx_tid: locale Λ
+  }.
+
+  Definition expr_at '(TpoolCtx K τ) (c: cfg Λ) (e: expr Λ) :=
+    from_locale c.1 τ = Some (ectx_fill K e).
+
+  Definition call_at {APP: expr Λ -> expr Λ -> expr Λ} tpc c (m a: val Λ) :=
+    expr_at tpc c (APP (language.of_val m) (language.of_val a)).
+
+  Definition return_at tpc c (r: val Λ) :=
+    expr_at tpc c (language.of_val r).
+
+  Definition nval_at tpc c :=
+    exists e, expr_at tpc c e /\ language.to_val e = None.
+
+  Lemma expr_at_in_locales {CNT: Countable (locale Λ)} tc c e
+    (EXPR: expr_at tc c e):
+    tpctx_tid tc ∈ locales_of_cfg c.
+  Proof using.
+    red in EXPR. destruct tc, c. simpl in *.
+    eapply locales_of_cfg_Some; eauto.
+  Qed.
+
+End ThreadPoolContext.
 
 
 Section TraceContext.
   Context `{EqDecision (locale Λ)}.
 
+  (* Record trace_ctx := TraceCtx { *)
+  (*   tctx_index: nat; *)
+  (*   tctx_tid: locale Λ; *)
+  (*   tctx_ctx: ectx Λ; *)
+  (* }. *)
   Record trace_ctx := TraceCtx {
     tctx_index: nat;
-    tctx_tid: locale Λ;
-    tctx_ctx: ectx Λ;
+    tctx_tpctx: @tpool_ctx Λ;
   }.
   
   Context (tr: extrace Λ). 
 
-  Definition expr_under '(TraceCtx i τ K) (e: expr Λ) :=
-    exists c, tr S!! i = Some c /\ from_locale c.1 τ = Some (ectx_fill K e).
+  (* Definition expr_under '(TraceCtx i τ K) (e: expr Λ) := *)
+  (*   exists c, tr S!! i = Some c /\ from_locale c.1 τ = Some (ectx_fill K e). *)
 
 End TraceContext.
